feat: offset constraints support for the `grind` tactic (#6603)
This PR implements support for offset constraints in the `grind` tactic.
Several features are still missing, such as constraint propagation and
support for offset equalities, but `grind` can already solve examples
like the following:

```lean
example (a b c : Nat) : a ≤ b → b + 2 ≤ c → a + 1 ≤ c := by
  grind
example (a b c : Nat) : a ≤ b → b ≤ c → a ≤ c := by
  grind
example (a b c : Nat) : a + 1 ≤ b → b + 1 ≤ c → a + 2 ≤ c := by
  grind
example (a b c : Nat) : a + 1 ≤ b → b + 1 ≤ c → a + 1 ≤ c := by
  grind
example (a b c : Nat) : a + 1 ≤ b → b ≤ c + 2 → a ≤ c + 1 := by
  grind
example (a b c : Nat) : a + 2 ≤ b → b ≤ c + 2 → a ≤ c := by
  grind
```

---------

Co-authored-by: Kim Morrison <scott.morrison@gmail.com>

src/Init/Grind/Offset.lean
@@ -7,159 +7,44 @@ prelude
 import Init.Core
 import Init.Omega
 
-namespace Lean.Grind.Offset
+namespace Lean.Grind
+def isLt (x y : Nat) : Bool := x < y
 
-abbrev Var := Nat
-abbrev Context := Lean.RArray Nat
+theorem Nat.le_ro (u w v k : Nat) : u ≤ w → w ≤ v + k → u ≤ v + k := by
+  omega
+theorem Nat.le_lo (u w v k : Nat) : u ≤ w → w + k ≤ v → u + k ≤ v := by
+  omega
+theorem Nat.lo_le (u w v k : Nat) : u + k ≤ w → w ≤ v → u + k ≤ v := by
+  omega
+theorem Nat.lo_lo (u w v k₁ k₂ : Nat) : u + k₁ ≤ w → w + k₂ ≤ v → u + (k₁ + k₂) ≤ v := by
+  omega
+theorem Nat.lo_ro_1 (u w v k₁ k₂ : Nat) : isLt k₂ k₁ = true → u + k₁ ≤ w → w ≤ v + k₂ → u + (k₁ - k₂) ≤ v := by
+  simp [isLt]; omega
+theorem Nat.lo_ro_2 (u w v k₁ k₂ : Nat) : u + k₁ ≤ w → w ≤ v + k₂ → u ≤ v + (k₂ - k₁) := by
+  omega
+theorem Nat.ro_le (u w v k : Nat) : u ≤ w + k → w ≤ v → u ≤ v + k := by
+  omega
+theorem Nat.ro_lo_1 (u w v k₁ k₂ : Nat) : u ≤ w + k₁ → w + k₂ ≤ v → u ≤ v + (k₁ - k₂) := by
+  omega
+theorem Nat.ro_lo_2 (u w v k₁ k₂ : Nat) : isLt k₁ k₂ = true → u ≤ w + k₁ → w + k₂ ≤ v → u + (k₂ - k₁) ≤ v := by
+  simp [isLt]; omega
+theorem Nat.ro_ro (u w v k₁ k₂ : Nat) : u ≤ w + k₁ → w ≤ v + k₂ → u ≤ v + (k₁ + k₂) := by
+  omega
 
-def fixedVar := 100000000 -- Any big number should work here
+theorem Nat.of_le_eq_false (u v : Nat) : ((u ≤ v) = False) → v + 1 ≤ u := by
+  simp; omega
+theorem Nat.of_lo_eq_false_1 (u v : Nat) : ((u + 1 ≤ v) = False) → v ≤ u := by
+  simp; omega
+theorem Nat.of_lo_eq_false (u v k : Nat) : ((u + k ≤ v) = False) → v ≤ u + (k-1) := by
+  simp; omega
+theorem Nat.of_ro_eq_false (u v k : Nat) : ((u ≤ v + k) = False) → v + (k+1) ≤ u := by
+  simp; omega
 
-def Var.denote (ctx : Context) (v : Var) : Nat :=
-  bif v == fixedVar then 1 else ctx.get v
+theorem Nat.unsat_le_lo (u v k : Nat) : isLt 0 k = true → u ≤ v → v + k ≤ u → False := by
+  simp [isLt]; omega
+theorem Nat.unsat_lo_lo (u v k₁ k₂ : Nat) : isLt 0 (k₁+k₂) = true → u + k₁ ≤ v → v + k₂ ≤ u → False := by
+  simp [isLt]; omega
+theorem Nat.unsat_lo_ro (u v k₁ k₂ : Nat) : isLt k₂ k₁ = true → u + k₁ ≤ v → v ≤ u + k₂ → False := by
+  simp [isLt]; omega
 
-structure Cnstr where
-  x : Var
-  y : Var
-  k : Nat  := 0
-  l : Bool := true
-  deriving Repr, DecidableEq, Inhabited
-
-def Cnstr.denote (c : Cnstr) (ctx : Context) : Prop :=
-  if c.l then
-    c.x.denote ctx + c.k ≤ c.y.denote ctx
-  else
-    c.x.denote ctx ≤ c.y.denote ctx + c.k
-
-def trivialCnstr : Cnstr := { x := 0, y := 0, k := 0, l := true }
-
-@[simp] theorem denote_trivial (ctx : Context) : trivialCnstr.denote ctx := by
-  simp [Cnstr.denote, trivialCnstr]
-
-def Cnstr.trans (c₁ c₂ : Cnstr) : Cnstr :=
-  if c₁.y = c₂.x then
-    let { x, k := k₁, l := l₁, .. } := c₁
-    let { y, k := k₂, l := l₂, .. } := c₂
-    match l₁, l₂ with
-    | false, false =>
-      { x, y, k := k₁ + k₂, l := false }
-    | false, true =>
-      if k₁ < k₂ then
-        { x, y, k := k₂ - k₁, l := true }
-      else
-        { x, y, k := k₁ - k₂, l := false }
-    | true, false =>
-      if k₁ < k₂ then
-        { x, y, k := k₂ - k₁, l := false }
-      else
-        { x, y, k := k₁ - k₂, l := true }
-    | true, true =>
-      { x, y, k := k₁ + k₂, l := true }
-  else
-    trivialCnstr
-
-@[simp] theorem Cnstr.denote_trans_easy (ctx : Context) (c₁ c₂ : Cnstr) (h : c₁.y ≠ c₂.x) : (c₁.trans c₂).denote ctx := by
-  simp [*, Cnstr.trans]
-
-@[simp] theorem Cnstr.denote_trans (ctx : Context) (c₁ c₂ : Cnstr) : c₁.denote ctx → c₂.denote ctx → (c₁.trans c₂).denote ctx := by
-  by_cases c₁.y = c₂.x
-  case neg => simp [*]
-  simp [trans, *]
-  let { x, k := k₁, l := l₁, .. } := c₁
-  let { y, k := k₂, l := l₂, .. } := c₂
-  simp_all; split
-  · simp [denote]; omega
-  · split <;> simp [denote] <;> omega
-  · split <;> simp [denote] <;> omega
-  · simp [denote]; omega
-
-def Cnstr.isTrivial (c : Cnstr) : Bool := c.x == c.y && c.k == 0
-
-theorem Cnstr.of_isTrivial (ctx : Context) (c : Cnstr) : c.isTrivial = true → c.denote ctx := by
-  cases c; simp [isTrivial]; intros; simp [*, denote]
-
-def Cnstr.isFalse (c : Cnstr) : Bool := c.x == c.y && c.k != 0 && c.l == true
-
-theorem Cnstr.of_isFalse (ctx : Context) {c : Cnstr} : c.isFalse = true → ¬c.denote ctx := by
-  cases c; simp [isFalse]; intros; simp [*, denote]; omega
-
-def Cnstrs := List Cnstr
-
-def Cnstrs.denoteAnd' (ctx : Context) (c₁ : Cnstr) (c₂ : Cnstrs) : Prop :=
-  match c₂ with
-  | [] => c₁.denote ctx
-  | c::cs => c₁.denote ctx ∧ Cnstrs.denoteAnd' ctx c cs
-
-theorem Cnstrs.denote'_trans (ctx : Context) (c₁ c : Cnstr) (cs : Cnstrs) : c₁.denote ctx → denoteAnd' ctx c cs → denoteAnd' ctx (c₁.trans c) cs := by
-  induction cs
-  next => simp [denoteAnd', *]; apply Cnstr.denote_trans
-  next c cs ih => simp [denoteAnd']; intros; simp [*]
-
-def Cnstrs.trans' (c₁ : Cnstr) (c₂ : Cnstrs) : Cnstr :=
-  match c₂ with
-  | [] => c₁
-  | c::c₂ => trans' (c₁.trans c) c₂
-
-@[simp] theorem Cnstrs.denote'_trans' (ctx : Context) (c₁ : Cnstr) (c₂ : Cnstrs) : denoteAnd' ctx c₁ c₂ → (trans' c₁ c₂).denote ctx := by
-  induction c₂ generalizing c₁
-  next => intros; simp_all [trans', denoteAnd']
-  next c cs ih => simp [denoteAnd']; intros; simp [trans']; apply ih; apply denote'_trans <;> assumption
-
-def Cnstrs.denoteAnd (ctx : Context) (c : Cnstrs) : Prop :=
-  match c with
-  | [] => True
-  | c::cs => denoteAnd' ctx c cs
-
-def Cnstrs.trans (c : Cnstrs) : Cnstr :=
-  match c with
-  | []    => trivialCnstr
-  | c::cs => trans' c cs
-
-theorem Cnstrs.of_denoteAnd_trans {ctx : Context} {c : Cnstrs} : c.denoteAnd ctx → c.trans.denote ctx := by
-  cases c <;> simp [*, trans, denoteAnd] <;> intros <;> simp [*]
-
-def Cnstrs.isFalse (c : Cnstrs) : Bool :=
-  c.trans.isFalse
-
-theorem Cnstrs.unsat' (ctx : Context) (c : Cnstrs) : c.isFalse = true → ¬ c.denoteAnd ctx := by
-  simp [isFalse]; intro h₁ h₂
-  have := of_denoteAnd_trans h₂
-  have := Cnstr.of_isFalse ctx h₁
-  contradiction
-
-/-- `denote ctx [c_1, ..., c_n] C` is `c_1.denote ctx → ... → c_n.denote ctx → C` -/
-def Cnstrs.denote (ctx : Context) (cs : Cnstrs) (C : Prop) : Prop :=
-  match cs with
-  | [] => C
-  | c::cs => c.denote ctx → denote ctx cs C
-
-theorem Cnstrs.not_denoteAnd'_eq (ctx : Context) (c : Cnstr) (cs : Cnstrs) (C : Prop) : (denoteAnd' ctx c cs → C) = denote ctx (c::cs) C := by
-  simp [denote]
-  induction cs generalizing c
-  next => simp [denoteAnd', denote]
-  next c' cs ih =>
-    simp [denoteAnd', denote, *]
-
-theorem Cnstrs.not_denoteAnd_eq (ctx : Context) (cs : Cnstrs) (C : Prop) : (denoteAnd ctx cs → C) = denote ctx cs C := by
-  cases cs
-  next => simp [denoteAnd, denote]
-  next c cs => apply not_denoteAnd'_eq
-
-def Cnstr.isImpliedBy (cs : Cnstrs) (c : Cnstr) : Bool :=
-  cs.trans == c
-
-/-! Main theorems used by `grind`. -/
-
-/-- Auxiliary theorem used by `grind` to prove that a system of offset inequalities is unsatisfiable. -/
-theorem Cnstrs.unsat (ctx : Context) (cs : Cnstrs) : cs.isFalse = true → cs.denote ctx False := by
-  intro h
-  rw [← not_denoteAnd_eq]
-  apply unsat'
-  assumption
-
-/-- Auxiliary theorem used by `grind` to prove an implied offset inequality. -/
-theorem Cnstrs.imp (ctx : Context) (cs : Cnstrs) (c : Cnstr) (h : c.isImpliedBy cs = true)  : cs.denote ctx (c.denote ctx) := by
-  rw [← eq_of_beq h]
-  rw [← not_denoteAnd_eq]
-  apply of_denoteAnd_trans
-
-end Lean.Grind.Offset
+end Lean.Grind
