src/Lean/Meta/Tactic/Grind/Arith/Offset.lean
@@ -1,0 +1,173 @@
+/-
+Copyright (c) 2025 Amazon.com, Inc. or its affiliates. All Rights Reserved.
+Released under Apache 2.0 license as described in the file LICENSE.
+Authors: Leonardo de Moura
+-/
+prelude
+import Init.Grind.Offset
+import Lean.Meta.Tactic.Grind.Types
+import Lean.Meta.Tactic.Grind.Arith.ProofUtil
+
+namespace Lean.Meta.Grind.Arith.Offset
+/-!
+This module implements a decision procedure for offset constraints of the form:
+```
+x + k ≤ y
+x ≤ y + k
+```
+where `k` is a numeral.
+Each constraint is represented as an edge in a weighted graph.
+The constraint `x + k ≤ y` is represented as a negative edge.
+The shortest path between two nodes in the graph corresponds to an implied inequality.
+When adding a new edge, the state is considered unsatisfiable if the new edge creates a negative cycle.
+An incremental Floyd-Warshall algorithm is used to find the shortest paths between all nodes.
+This module can also handle offset equalities of the form `x + k = y` by representing them with two edges:
+```
+x + k ≤ y
+y ≤ x + k
+```
+The main advantage of this module over a full linear integer arithmetic procedure is
+its ability to efficiently detect all implied equalities and inequalities.
+-/
+
+def get' : GoalM State := do
+  return (← get).arith.offset
+
+@[inline] def modify' (f : State → State) : GoalM Unit := do
+  modify fun s => { s with arith.offset := f s.arith.offset }
+
+def mkNode (expr : Expr) : GoalM NodeId := do
+  if let some nodeId := (← get').nodeMap.find? { expr } then
+    return nodeId
+  let nodeId : NodeId := (← get').nodes.size
+  trace[grind.offset.internalize.term] "{expr} ↦ #{nodeId}"
+  modify' fun s => { s with
+    nodes   := s.nodes.push expr
+    nodeMap := s.nodeMap.insert { expr } nodeId
+    sources := s.sources.push {}
+    targets := s.targets.push {}
+    proofs  := s.proofs.push {}
+  }
+  return nodeId
+
+private def getDist? (u v : NodeId) : GoalM (Option Int) := do
+  return (← get').targets[u]!.find? v
+
+private def getProof? (u v : NodeId) : GoalM (Option ProofInfo) := do
+  return (← get').proofs[u]!.find? v
+
+partial def extractProof (u v : NodeId) : GoalM Expr := do
+  go (← getProof? u v).get!
+where
+  go (p : ProofInfo) : GoalM Expr := do
+    if u == p.w then
+      return p.proof
+    else
+      let p' := (← getProof? u p.w).get!
+      go (mkTrans (← get').nodes p' p v)
+
+private def setUnsat (u v : NodeId) (kuv : Int) (huv : Expr) (kvu : Int) : GoalM Unit := do
+  assert! kuv + kvu < 0
+  let hvu ← extractProof v u
+  let u := (← get').nodes[u]!
+  let v := (← get').nodes[v]!
+  if kuv == 0 then
+    assert! kvu < 0
+    closeGoal (mkApp6 (mkConst ``Grind.Nat.unsat_le_lo) u v (toExpr (-kvu).toNat) rfl_true huv hvu)
+  else if kvu == 0 then
+    assert! kuv < 0
+    closeGoal (mkApp6 (mkConst ``Grind.Nat.unsat_le_lo) v u (toExpr (-kuv).toNat) rfl_true hvu huv)
+  else if kuv < 0 then
+    if kvu > 0 then
+      closeGoal (mkApp7 (mkConst ``Grind.Nat.unsat_lo_ro) u v (toExpr (-kuv).toNat) (toExpr kvu.toNat) rfl_true huv hvu)
+    else
+      assert! kvu < 0
+      closeGoal (mkApp7 (mkConst ``Grind.Nat.unsat_lo_lo) u v (toExpr (-kuv).toNat) (toExpr (-kvu).toNat) rfl_true huv hvu)
+  else
+    assert! kuv > 0 && kvu < 0
+    closeGoal (mkApp7 (mkConst ``Grind.Nat.unsat_lo_ro) v u (toExpr (-kvu).toNat) (toExpr kuv.toNat) rfl_true hvu huv)
+
+private def setDist (u v : NodeId) (k : Int) : GoalM Unit := do
+  trace[grind.offset.dist] "{({ a := u, b := v, k : Cnstr NodeId})}"
+  modify' fun s => { s with
+    targets := s.targets.modify u fun es => es.insert v k
+    sources := s.sources.modify v fun es => es.insert u k
+  }
+
+private def setProof (u v : NodeId) (p : ProofInfo) : GoalM Unit := do
+  modify' fun s => { s with
+    proofs := s.proofs.modify u fun es => es.insert v p
+  }
+
+@[inline]
+private def forEachSourceOf (u : NodeId) (f : NodeId → Int → GoalM Unit) : GoalM Unit := do
+  (← get').sources[u]!.forM f
+
+@[inline]
+private def forEachTargetOf (u : NodeId) (f : NodeId → Int → GoalM Unit) : GoalM Unit := do
+  (← get').targets[u]!.forM f
+
+private def isShorter (u v : NodeId) (k : Int) : GoalM Bool := do
+  if let some k' ← getDist? u v then
+    return k < k'
+  else
+    return true
+
+private def updateIfShorter (u v : NodeId) (k : Int) (w : NodeId) : GoalM Unit := do
+  if (← isShorter u v k) then
+    setDist u v k
+    setProof u v (← getProof? w v).get!
+
+def addEdge (u : NodeId) (v : NodeId) (k : Int) (p : Expr) : GoalM Unit := do
+  if (← isInconsistent) then return ()
+  if let some k' ← getDist? v u then
+    if k'+k < 0 then
+      setUnsat u v k p k'
+      return ()
+  if (← isShorter u v k) then
+    setDist u v k
+    setProof u v { w := u, k, proof := p }
+    update
+where
+  update : GoalM Unit := do
+    forEachTargetOf v fun j k₂ => do
+      /- Check whether new path: `u -(k)-> v -(k₂)-> j` is shorter -/
+      updateIfShorter u j (k+k₂) v
+    forEachSourceOf u fun i k₁ => do
+      /- Check whether new path: `i -(k₁)-> u -(k)-> v` is shorter -/
+      updateIfShorter i v (k₁+k) u
+      forEachTargetOf v fun j k₂ => do
+        /- Check whether new path: `i -(k₁)-> u -(k)-> v -(k₂) -> j` is shorter -/
+        updateIfShorter i j (k₁+k+k₂) v
+
+def traceDists : GoalM Unit := do
+  let s ← get'
+  for u in [:s.targets.size], es in s.targets.toArray do
+    for (v, k) in es do
+      trace[grind.offset.dist] "#{u} -({k})-> #{v}"
+
+def Cnstr.toExpr (c : Cnstr NodeId) : GoalM Expr := do
+  let a := (← get').nodes[c.a]!
+  let b := (← get').nodes[c.b]!
+  let mk := if c.le then mkNatLE else mkNatEq
+  if c.k == 0 then
+    return mk a b
+  else if c.k < 0 then
+    return mk (mkNatAdd a (Lean.toExpr ((-c.k).toNat))) b
+  else
+    return mk a (mkNatAdd b (Lean.toExpr c.k.toNat))
+
+def checkInvariants : GoalM Unit := do
+  let s ← get'
+  for u in [:s.targets.size], es in s.targets.toArray do
+    for (v, k) in es do
+      let c : Cnstr NodeId := { a := u, b := v, k }
+      trace[grind.debug.offset] "{c}"
+      let p ← extractProof u v
+      trace[grind.debug.offset.proof] "{p} : {← inferType p}"
+      check p
+      unless (← withDefault <| isDefEq (← inferType p) (← Cnstr.toExpr c)) do
+        trace[grind.debug.offset.proof] "failed: {← inferType p} =?= {← Cnstr.toExpr c}"
+        unreachable!
+
+end Lean.Meta.Grind.Arith.Offset
