src/Lean/Meta/Tactic/Grind/Types.lean
@@ -13,16 +13,13 @@ import Lean.Meta.CongrTheorems
 import Lean.Meta.AbstractNestedProofs
 import Lean.Meta.Tactic.Simp.Types
 import Lean.Meta.Tactic.Util
+import Lean.Meta.Tactic.Grind.ENodeKey
 import Lean.Meta.Tactic.Grind.Canon
 import Lean.Meta.Tactic.Grind.Attr
+import Lean.Meta.Tactic.Grind.Arith.Types
 import Lean.Meta.Tactic.Grind.EMatchTheorem
 
 namespace Lean.Meta.Grind
-
-@[inline] def isSameExpr (a b : Expr) : Bool :=
-  -- It is safe to use pointer equality because we hashcons all expressions
-  -- inserted into the E-graph
-  unsafe ptrEq a b
 
 /-- We use this auxiliary constant to mark delayed congruence proofs. -/
 def congrPlaceholderProof := mkConst (Name.mkSimple "[congruence]")
@@ -224,20 +221,6 @@ structure NewEq where
   proof : Expr
   isHEq : Bool
 
-/--
-Key for the `ENodeMap` and `ParentMap` map.
-We use pointer addresses and rely on the fact all internalized expressions
-have been hash-consed, i.e., we have applied `shareCommon`.
--/
-private structure ENodeKey where
-  expr : Expr
-
-instance : Hashable ENodeKey where
-  hash k := unsafe (ptrAddrUnsafe k.expr).toUInt64
-
-instance : BEq ENodeKey where
-  beq k₁ k₂ := isSameExpr k₁.expr k₂.expr
-
 abbrev ENodeMap := PHashMap ENodeKey ENode
 
 /--
@@ -368,6 +351,8 @@ structure Goal where
   gmt          : Nat := 0
   /-- Next unique index for creating ENodes -/
   nextIdx      : Nat := 0
+  /-- State of arithmetic procedures -/
+  arith        : Arith.State := {}
   /-- Active theorems that we have performed ematching at least once. -/
   thms         : PArray EMatchTheorem := {}
   /-- Active theorems that we have not performed any round of ematching yet. -/
